while_not_b.ec
@@ -4,14 +4,13 @@ require import Int.
 
 type rt.
 
-op myd : rt distr.
 op MyP : rt -> bool.
 
 
 
 module M = {
   var c : int
-  proc whp(s : int, e : int, r : rt) = {
+  proc whp(myd : rt distr, s : int, e : int, r : rt) = {
     c <- s;
     while(c <= e /\ !MyP r){
      r <$ myd;
@@ -20,9 +19,9 @@ module M = {
     return r;
   }
 
-  proc whp_if_end(s : int, e : int, r : rt) = {
+  proc whp_if_end(myd : rt distr, s : int, e : int, r : rt) = {
     var ri : rt;
-    ri <- whp(s,e,r);     
+    ri <- whp(myd, s,e,r);     
     if(c <= e + 1 /\ !MyP ri){
       ri <$ myd;
       c <- c + 1;
@@ -33,14 +32,14 @@ module M = {
 
 
 lemma whp_split_if_end :  
-  equiv[ M.whp ~ M.whp_if_end : ={s,r} /\ e{1} - 1 = e{2}
+  equiv[ M.whp ~ M.whp_if_end : ={myd, s,r} /\ e{1} - 1 = e{2}
         ==> ={res,M.c} ].
 proof. proc.
 inline*. sp. 
 splitwhile{1} 1 : M.c  <= (e - 1) .
-seq  1 1 : (={M.c} /\ r{1} = r0{2} /\ e0{2} = e{2}
+seq  1 1 : (={M.c} /\ r{1} = r0{2} /\ myd{1} = myd0{2} /\ e0{2} = e{2} /\ myd0{2} = myd{2}
    /\ e{1} - 1 = e0{2} /\ (!MyP r{1} => (e{1} - 1) < M.c{1} )).
-while (={M.c} /\ r{1} = r0{2} /\ e0{2} = e{2}
+while (={M.c,myd} /\ r{1} = r0{2} /\ myd{1} = myd0{2} /\ e0{2} = e{2}
    /\ e{1} - 1 = e0{2} ).
 wp. rnd. skip. progress. smt.  skip. progress. smt. smt.
 sp. simplify.
@@ -57,13 +56,13 @@ rcondf {1} 1. progress. skip. progress.
 qed.
 
 
-lemma whp_split_if_end' s e r p P :  
-  (phoare [ M.whp_if_end : arg = (s,e,r) ==> P res ] = p)
-   => phoare [ M.whp : arg = (s,e+1,r) ==> P res ] = p.
+lemma whp_split_if_end' s e r p P d :  
+  (phoare [ M.whp_if_end : arg = (d,s,e,r) ==> P res ] = p)
+   => phoare [ M.whp : arg = (d,s,e+1,r) ==> P res ] = p.
 proof. progress. bypr.
 progress.
-have <-: Pr[M.whp_if_end(s{m}, e{m}, r{m}) @ &m : P res] = p.
-byphoare (_: arg = (s{m}, e{m}, r{m}) ==> _).
+have <-: Pr[M.whp_if_end(d{m}, s{m}, e{m}, r{m}) @ &m : P res] = p.
+byphoare (_: arg = (d{m}, s{m}, e{m}, r{m}) ==> _).
 conseq H. auto. auto. byequiv.
 conseq whp_split_if_end. smt. auto. auto. auto.
 qed.
@@ -73,23 +72,23 @@ lemma lll (b a c : real) : a <= b => b <= c => a <= c.
 smt. qed.
 
     
-lemma whp_split_if_end_le s e r p P :  
-  (phoare [ M.whp_if_end : arg = (s,e,r) ==> P res ] <= p)
-   => phoare [ M.whp : arg = (s,e+1,r) ==> P res ] <= p.
+lemma whp_split_if_end_le s e r p myd P :  
+  (phoare [ M.whp_if_end : arg = (myd,s,e,r) ==> P res ] <= p)
+   => phoare [ M.whp : arg = (myd,s,e+1,r) ==> P res ] <= p.
 proof. progress. bypr.
 progress.
-have zz : Pr[M.whp_if_end(s{m}, e{m}, r{m}) @ &m : P res] <= p.
-byphoare (_: arg = (s{m}, e{m}, r{m}) ==> _).
+have zz : Pr[M.whp_if_end(myd{m},s{m}, e{m}, r{m}) @ &m : P res] <= p.
+byphoare (_: arg = (myd{m},s{m}, e{m}, r{m}) ==> _).
 conseq H. auto. auto. 
-apply (lll Pr[M.whp_if_end(s, e, r) @ &m : P res] ).
+apply (lll Pr[M.whp_if_end(myd,s, e, r) @ &m : P res] ).
 byequiv.
  conseq whp_split_if_end. smt. auto. auto. auto. apply zz.
 qed.
 
 
 
-lemma asdsad r:  MyP r = false => forall e, 0 <= e => 
-  phoare[ M.whp_if_end : arg = (1,e,r) ==> !MyP res ] = ((1%r/2%r) ^ (e+1)).
+lemma asdsad r myd:  MyP r = false => forall e, 0 <= e => 
+  phoare[ M.whp_if_end : arg = (myd, 1,e,r) ==> !MyP res ] = ((1%r/2%r) ^ (e+1)).
 proof. move => ipr. apply ge0ind. smt.
 progress. simplify.
   progress. proc.
@@ -100,8 +99,8 @@ rcondt 1. skip. progress. smt.
 swap 1 1.  rnd.  simplify.
 wp.  skip.  progress. admit.
 progress. proc.
-  have phf: phoare[ M.whp : arg = (1, n+1, r) ==> !MyP res] = (inv 2%r ^(n+1)).
- apply (whp_split_if_end' 1 n r ((inv 2%r)^(n+1)) (fun x => !MyP x) (H0 H) ).
+  have phf: phoare[ M.whp : arg = (myd, 1, n+1, r) ==> !MyP res] = (inv 2%r ^(n+1)).
+ apply (whp_split_if_end'  1 n r  ((inv 2%r)^(n+1)) (fun x => !MyP x) myd (H0 H) ).
 seq 1 : (!MyP ri) (inv 2%r ^(n+1)) (1%r/2%r) 1%r 0%r (!MyP ri => M.c <= e + 1).
 inline*. sp.
 seq 1 :  (!MyP r0 => M.c <= e + 1).
@@ -119,8 +118,8 @@ simplify. skip. auto. smt.
 qed.
 
 
-lemma asdsad_le r:  MyP r = false => forall e, 0 <= e => 
-  phoare[ M.whp_if_end : arg = (1,e,r) ==> !MyP res ]
+lemma asdsad_le r d:  MyP r = false => forall e, 0 <= e => 
+  phoare[ M.whp_if_end : arg = (d,1,e,r) ==> !MyP res ]
      <= ((1%r/2%r) ^ (e+1)).
 proof. move => ipr. apply ge0ind. smt.
 progress. simplify.
@@ -132,8 +131,8 @@ rcondt 1. skip. progress. smt.
 swap 1 1.  rnd.  simplify.
 wp.  skip.  progress. admit.
 progress. proc.
-  have phf: phoare[ M.whp : arg = (1, n+1, r) ==> !MyP res] <= (inv 2%r ^(n+1)).
- apply (whp_split_if_end_le 1 n r ((inv 2%r)^(n+1)) (fun x => !MyP x) (H0 H) ).
+  have phf: phoare[ M.whp : arg = (d,1, n+1, r) ==> !MyP res] <= (inv 2%r ^(n+1)).
+ apply (whp_split_if_end_le 1 n r ((inv 2%r)^(n+1)) d (fun x => !MyP x) (H0 H) ).
 seq 1 : (!MyP ri) (inv 2%r ^(n+1)) (1%r/2%r) 1%r 0%r (!MyP ri => M.c <= e + 1).
 inline*. sp.
 seq 1 :  (!MyP r0 => M.c <= e + 1).
@@ -151,10 +150,10 @@ simplify. skip. auto. smt.
 qed.
 
 
-lemma asdsadq r:  MyP r = false => forall e, 0 <= e =>
-  phoare[ M.whp : arg = (1,e+1,r) ==> !MyP res ] = ((1%r/2%r) ^ (e+1)).
+lemma asdsadq r d:  MyP r = false => forall e, 0 <= e =>
+  phoare[ M.whp : arg = (d,1,e+1,r) ==> !MyP res ] = ((1%r/2%r) ^ (e+1)).
 progress.
-have fact1  : phoare[ M.whp_if_end : arg = (1,e,r) ==> !MyP res ] = ((1%r/2%r) ^ (e+1)).
-apply (asdsad r H e H0). auto.
-conseq (whp_split_if_end' 1 e r ((inv 2%r)^(e+1)) (fun x => !MyP x) fact1).
+have fact1  : phoare[ M.whp_if_end : arg = (d,1,e,r) ==> !MyP res ] = ((1%r/2%r) ^ (e+1)).
+apply (asdsad r d H e H0). auto.
+conseq (whp_split_if_end' 1 e r ((inv 2%r)^(e+1)) (fun x => !MyP x) d fact1).
 qed.
