mywhille.ec
@@ -1,0 +1,162 @@
+pragma Goals:printall.
+require import Int.
+
+type rrt, irt.
+
+
+module type Run = {
+  proc run(i:irt) : rrt
+}.                                  
+
+module W(A : Run) = {
+  var c : int
+  proc whp(p : rrt -> bool, i : irt, s : int, e : int, r : rrt) = {
+    c <- s;
+    while(c <= e /\ !p r){
+     r <- A.run(i);
+     c <- c + 1;
+    }
+    return r;
+  }
+
+  proc if_whp(p : rrt -> bool, i : irt, s : int, e : int, r : rrt) = {
+    c <- s;
+    if(c <= e /\ !p r){
+     r <- A.run(i);
+     c <- c + 1;
+    }
+    r <- whp(p,i,W.c,e,r);
+    return r;
+  }
+
+  proc whp_if(p : rrt -> bool, i : irt, s : int, e : int, r : rrt) = {
+    c <- s;
+    r <- whp(p,i,s,e-1,r);
+    if(c <= e /\ !p r){
+     r <- A.run(i);
+     c <- c + 1;
+    }
+    return r;
+  }
+
+  proc whp_split(p : rrt -> bool, i : irt, s : int, m : int, e : int, r : rrt) = {
+    c <- s;
+    r <- whp(p,i,s,m,r);
+    r <- whp(p,i,W.c,e,r);
+    return r;
+  }
+  
+}.
+
+section.
+
+declare module A : Run {W}.
+
+axiom A_ll : islossless A.run.
+
+lemma if_whp_prop : 
+  equiv [ W(A).whp ~ W(A).if_whp : ={glob W, glob A, arg} ==>  ={glob W, glob A, res} ].
+proc. inline*.
+unroll {1} 2.
+sp.
+if. progress.
+seq 2 8 : (={glob A, glob W} /\ e{1} = e0{2} /\ p{1} = p0{2} /\ r{1} = r0{2} /\ i{1} = i0{2} 
+  /\ e{2} = e0{2} /\ p{2} = p0{2} /\ r{2} = r0{2} /\ i{2} = i0{2} ).
+wp.  call (_:true). skip. progress.
+wp.
+ while (={glob A, glob W} /\ e{1} = e0{2} /\ p{1} = p0{2} /\ r{1} = r0{2} /\ i{1} = i0{2} ).
+wp.
+call (_: true). skip. progress.
+skip. progress.
+sp.
+rcondf {1} 1. progress.
+rcondf {2} 1. progress. wp. skip. progress. 
+qed.
+
+
+lemma whp_if_prop : 
+  equiv [ W(A).whp ~ W(A).whp_if : s{2} <= e{2} /\ ={glob W, glob A, arg} ==>  ={glob W, glob A, res} ].
+proc.
+inline*. sp. 
+splitwhile {1} 1 : (W.c <= e-1).
+seq 1 1 : (={W.c, glob A,e,p,i} /\ e{1} = e0{2} + 1  /\ p{1} = p0{2} /\ r{1} = r0{2} /\ i{1} = i0{2} /\ (! p r => W.c = e){1}).
+while (={W.c, glob A,e,p,i} /\ e{1} = e0{2} + 1 /\ p{1} = p0{2}  /\ r{1} = r0{2} /\ i{1} = i0{2} /\ (! p r => W.c <= e){1}).
+wp. call (_:true). skip. progress.
+smt. smt.
+skip. progress. smt.
+sp.
+unroll {1} 1.
+seq 1 1 : (={glob A, W.c,e,p,r,i} /\ (! p{1} r{1} => W.c{1} = e{1}+1)). 
+if. progress. wp. call (_:true). skip. progress. smt. skip. progress. smt.
+rcondf {1} 1. progress. skip. progress. smt. skip. progress.
+qed.
+
+
+lemma whp_split_prop : 
+  equiv [ W(A).whp ~ W(A).whp_split : m{2} <= e{2}  /\ ={glob W, glob A, p, i, s, e, r}
+        ==>  ={glob W, glob A, res} ].
+proc.  inline*.
+exists* m{2}. elim*. progress.
+splitwhile {1} 2 : (W.c <= m_R).      
+sp.
+seq 1 1 : (={glob A, W.c,p,i,e} /\ m_R = m{2} /\ m{2} <= e{2} /\ e0{2} = m_R /\ r{1} = r0{2} /\ p{1} = p0{2} /\ i{1} = i0{2}).
+while (={glob A, W.c,p,i,e} /\ m_R = m{2}  /\ m{2} <= e{2} /\ e0{2} = m_R /\ r{1} = r0{2} /\ p{1} = p0{2} /\ i{1} = i0{2}).
+wp. call (_:true). skip. progress. smt. 
+skip. progress. smt.
+sp. 
+wp.
+while (={glob A, W.c,p,i,e} /\ m_R = m{2}  /\ e{2} = e1{2} /\ m{2} <= e{2} /\ e0{2} = m_R /\ r{1} = r1{2} /\ p{1} = p1{2} /\ i{1} = i1{2}).
+wp. call (_:true). skip. progress. 
+skip. progress.
+qed.
+
+
+
+
+
+local lemma whp_premat_1 &m pa ia sa ea ra ja : sa <= ja =>
+  Pr[ W(A).whp(pa,ia,sa,ja,ra) @ &m : W.c = ja /\ pa res ]
+   =   Pr[ W(A).whp_split(pa,ia,sa,ja,ea,ra) @ &m : W.c = ja /\ pa res ].
+proof. move => hp.
+byequiv.
+proc*. 
+inline W(A).whp_split. sp. 
+seq 1 1 : (={glob A, glob W} /\ p{1} = pa /\ p0{2} = pa /\ r0{1} = r1{2} /\ p{1} = p0{2} /\ e{1} = ja /\ i{1} = i0{2} /\ s{1} = s0{2} /\ (!p r0 => W.c = e + 1){1} ).
+inline*.  sp. wp.
+while (={glob A, glob W} /\ (e0,p0,r1,i0){1} = (e1,p1,r2,i1){2} /\ (!p0 r1 => W.c <= e0 + 1){1}). wp. call (_:true). skip. progress.
+smt. skip. progress. smt.
+smt.
+inline*.  sp. 
+case (pa r0{1}).
+rcondf {2} 1. progress.  skip. progress. smt.
+wp. skip. progress. wp. 
+conseq (_:   (! pa r0{1}) /\ W.c{1} = ja + 1  /\ W.c{2} = W.c{1} ==> _ ). progress. smt.
+seq 0 1 : (! pa r0{1} /\ ja < W.c{2}) .
+while {2}  ( ja < W.c{2}) (e1{2} + 1 - W.c{2}). progress.
+wp.  call (_: true ==> true). apply A_ll.
+skip. progress. smt. smt. skip. progress.
+smt. smt. 
+skip. smt. 
+auto. auto.
+qed.
+
+
+lemma whp_cap &m p i s ea r ja :  s <= ja => ja <= ea =>
+   Pr[ W(A).whp(p,i,s,ea,r) @ &m : W.c = ja /\ p res ] 
+   =   Pr[ W(A).whp(p,i,s,ja,r) @ &m : W.c = ja /\ p res ].
+move => sjp jap.
+have ->:  Pr[ W(A).whp(p,i,s,ja,r) @ &m : W.c = ja /\ p res ] 
+  =  Pr[ W(A).whp_split(p,i,s,ja,ea,r) @ &m : W.c = ja /\ p res ] .
+ rewrite - whp_premat_1. auto. 
+auto.
+byequiv (_: ={p,i,s,e,r, glob A, glob W} /\ e{2} = ea /\ m{2} = ja /\ m{2} <= e{2} ==> _) .
+conseq whp_split_prop.
+progress.
+progress.
+progress.
+auto.
+qed.
+
+
+end section.
+  
